Adding initial support for observations to the definition of wp for later prophecy support

theories/heap_lang/lang.v
@@ -108,6 +108,8 @@ Inductive val :=
 
 Bind Scope val_scope with val.
 
+Inductive observation := prophecy_observation_todo.
+
 Fixpoint of_val (v : val) : expr :=
   match v with
   | RecV f x e => Rec f x e
@@ -199,7 +201,7 @@ Proof.
   end) (λ l, match l with
   | (inl (inl n), None) => LitInt n | (inl (inr b), None) => LitBool b
   | (inr (inl ()), None) => LitUnit | (inr (inr l), None) => LitLoc l
-  | (_, Some p) => LitProphecy p                                                                 
+  | (_, Some p) => LitProphecy p
   end) _); by intros [].
 Qed.
 Instance un_op_finite : Countable un_op.
@@ -415,62 +417,61 @@ Definition vals_cas_compare_safe (vl v1 : val) : Prop :=
   val_is_unboxed vl ∨ val_is_unboxed v1.
 Arguments vals_cas_compare_safe !_ !_ /.
 
-Inductive head_step : expr → state → expr → state → list (expr) → Prop :=
+Inductive head_step : expr → state → option observation -> expr → state → list (expr) → Prop :=
   | BetaS f x e1 e2 v2 e' σ :
      to_val e2 = Some v2 →
      Closed (f :b: x :b: []) e1 →
      e' = subst' x (of_val v2) (subst' f (Rec f x e1) e1) →
-     head_step (App (Rec f x e1) e2) σ e' σ []
+     head_step (App (Rec f x e1) e2) σ None e' σ []
   | UnOpS op e v v' σ :
      to_val e = Some v →
      un_op_eval op v = Some v' →
-     head_step (UnOp op e) σ (of_val v') σ []
+     head_step (UnOp op e) σ None (of_val v') σ []
   | BinOpS op e1 e2 v1 v2 v' σ :
      to_val e1 = Some v1 → to_val e2 = Some v2 →
      bin_op_eval op v1 v2 = Some v' →
-     head_step (BinOp op e1 e2) σ (of_val v') σ []
+     head_step (BinOp op e1 e2) σ None (of_val v') σ []
   | IfTrueS e1 e2 σ :
-     head_step (If (Lit $ LitBool true) e1 e2) σ e1 σ []
+     head_step (If (Lit $ LitBool true) e1 e2) σ None e1 σ []
   | IfFalseS e1 e2 σ :
-     head_step (If (Lit $ LitBool false) e1 e2) σ e2 σ []
+     head_step (If (Lit $ LitBool false) e1 e2) σ None e2 σ []
   | FstS e1 v1 e2 v2 σ :
      to_val e1 = Some v1 → to_val e2 = Some v2 →
-     head_step (Fst (Pair e1 e2)) σ e1 σ []
+     head_step (Fst (Pair e1 e2)) σ None e1 σ []
   | SndS e1 v1 e2 v2 σ :
      to_val e1 = Some v1 → to_val e2 = Some v2 →
-     head_step (Snd (Pair e1 e2)) σ e2 σ []
+     head_step (Snd (Pair e1 e2)) σ None e2 σ []
   | CaseLS e0 v0 e1 e2 σ :
      to_val e0 = Some v0 →
-     head_step (Case (InjL e0) e1 e2) σ (App e1 e0) σ []
+     head_step (Case (InjL e0) e1 e2) σ None (App e1 e0) σ []
   | CaseRS e0 v0 e1 e2 σ :
      to_val e0 = Some v0 →
-     head_step (Case (InjR e0) e1 e2) σ (App e2 e0) σ []
+     head_step (Case (InjR e0) e1 e2) σ None (App e2 e0) σ []
   | ForkS e σ:
-     head_step (Fork e) σ (Lit LitUnit) σ [e]
+     head_step (Fork e) σ None (Lit LitUnit) σ [e]
   | AllocS e v σ l :
      to_val e = Some v → σ !! l = None →
-     head_step (Alloc e) σ (Lit $ LitLoc l) (<[l:=v]>σ) []
+     head_step (Alloc e) σ None (Lit $ LitLoc l) (<[l:=v]>σ) []
   | LoadS l v σ :
      σ !! l = Some v →
-     head_step (Load (Lit $ LitLoc l)) σ (of_val v) σ []
+     head_step (Load (Lit $ LitLoc l)) σ None (of_val v) σ []
   | StoreS l e v σ :
      to_val e = Some v → is_Some (σ !! l) →
-     head_step (Store (Lit $ LitLoc l) e) σ (Lit LitUnit) (<[l:=v]>σ) []
+     head_step (Store (Lit $ LitLoc l) e) σ None (Lit LitUnit) (<[l:=v]>σ) []
   | CasFailS l e1 v1 e2 v2 vl σ :
      to_val e1 = Some v1 → to_val e2 = Some v2 →
      σ !! l = Some vl → vl ≠ v1 →
      vals_cas_compare_safe vl v1 →
-     head_step (CAS (Lit $ LitLoc l) e1 e2) σ (Lit $ LitBool false) σ []
+     head_step (CAS (Lit $ LitLoc l) e1 e2) σ None (Lit $ LitBool false) σ []
   | CasSucS l e1 v1 e2 v2 σ :
      to_val e1 = Some v1 → to_val e2 = Some v2 →
      σ !! l = Some v1 →
      vals_cas_compare_safe v1 v1 →
-     head_step (CAS (Lit $ LitLoc l) e1 e2) σ (Lit $ LitBool true) (<[l:=v2]>σ) []
+     head_step (CAS (Lit $ LitLoc l) e1 e2) σ None (Lit $ LitBool true) (<[l:=v2]>σ) []
   | FaaS l i1 e2 i2 σ :
      to_val e2 = Some (LitV (LitInt i2)) →
      σ !! l = Some (LitV (LitInt i1)) →
-     head_step (FAA (Lit $ LitLoc l) e2) σ (Lit $ LitInt i1) (<[l:=LitV (LitInt (i1 + i2))]>σ) [].
-
+     head_step (FAA (Lit $ LitLoc l) e2) σ None (Lit $ LitInt i1) (<[l:=LitV (LitInt (i1 + i2))]>σ) [].
 
 (** Basic properties about the language *)
 Instance fill_item_inj Ki : Inj (=) (=) (fill_item Ki).
@@ -480,11 +481,11 @@ Lemma fill_item_val Ki e :
   is_Some (to_val (fill_item Ki e)) → is_Some (to_val e).
 Proof. intros [v ?]. destruct Ki; simplify_option_eq; eauto. Qed.
 
-Lemma val_head_stuck e1 σ1 e2 σ2 efs : head_step e1 σ1 e2 σ2 efs → to_val e1 = None.
+Lemma val_head_stuck e1 σ1 κ e2 σ2 efs : head_step e1 σ1 κ e2 σ2 efs → to_val e1 = None.
 Proof. destruct 1; naive_solver. Qed.
 
-Lemma head_ctx_step_val Ki e σ1 e2 σ2 efs :
-  head_step (fill_item Ki e) σ1 e2 σ2 efs → is_Some (to_val e).
+Lemma head_ctx_step_val Ki e σ1 κ e2 σ2 efs :
+  head_step (fill_item Ki e) σ1 κ e2 σ2 efs → is_Some (to_val e).
 Proof. destruct Ki; inversion_clear 1; simplify_option_eq; by eauto. Qed.
 
 Lemma fill_item_no_val_inj Ki1 Ki2 e1 e2 :
@@ -499,7 +500,7 @@ Qed.
 
 Lemma alloc_fresh e v σ :
   let l := fresh (dom (gset loc) σ) in
-  to_val e = Some v → head_step (Alloc e) σ (Lit (LitLoc l)) (<[l:=v]>σ) [].
+  to_val e = Some v → head_step (Alloc e) σ None (Lit (LitLoc l)) (<[l:=v]>σ) [].
 Proof. by intros; apply AllocS, (not_elem_of_dom (D:=gset loc)), is_fresh. Qed.
 
 (* Misc *)
