theories/program_logic/lifting.v
@@ -15,7 +15,7 @@ Lemma wp_lift_step_fupd s E Φ e1 :
   to_val e1 = None →
   (∀ σ1, state_interp σ1 ={E,∅}=∗
     ⌜if s is NotStuck then reducible e1 σ1 else True⌝ ∗
-    ∀ e2 σ2 efs, ⌜prim_step e1 σ1 e2 σ2 efs⌝ ={∅,∅,E}▷=∗
+    ∀ κ e2 σ2 efs, ⌜prim_step e1 σ1 κ e2 σ2 efs⌝ ={∅,∅,E}▷=∗
       state_interp σ2 ∗ WP e2 @ s; E {{ Φ }} ∗ [∗ list] ef ∈ efs, WP ef @ s; ⊤ {{ _, True }})
   ⊢ WP e1 @ s; E {{ Φ }}.
 Proof.
@@ -30,7 +30,7 @@ Lemma wp_lift_stuck E Φ e :
 Proof.
   rewrite wp_unfold /wp_pre=>->. iIntros "H" (σ1) "Hσ".
   iMod ("H" with "Hσ") as %[? Hirr]. iModIntro. iSplit; first done.
-  iIntros (e2 σ2 efs) "% !> !>". by case: (Hirr e2 σ2 efs).
+  iIntros (κ e2 σ2 efs) "% !> !>". by case: (Hirr κ e2 σ2 efs).
 Qed.
 
 (** Derived lifting lemmas. *)
@@ -38,7 +38,7 @@ Lemma wp_lift_step s E Φ e1 :
   to_val e1 = None →
   (∀ σ1, state_interp σ1 ={E,∅}=∗
     ⌜if s is NotStuck then reducible e1 σ1 else True⌝ ∗
-    ▷ ∀ e2 σ2 efs, ⌜prim_step e1 σ1 e2 σ2 efs⌝ ={∅,E}=∗
+    ▷ ∀ κ e2 σ2 efs, ⌜prim_step e1 σ1 κ e2 σ2 efs⌝ ={∅,E}=∗
       state_interp σ2 ∗ WP e2 @ s; E {{ Φ }} ∗ [∗ list] ef ∈ efs, WP ef @ s; ⊤ {{ _, True }})
   ⊢ WP e1 @ s; E {{ Φ }}.
 Proof.
@@ -48,8 +48,8 @@ Qed.
 
 Lemma wp_lift_pure_step `{Inhabited (state Λ)} s E E' Φ e1 :
   (∀ σ1, if s is NotStuck then reducible e1 σ1 else to_val e1 = None) →
-  (∀ σ1 e2 σ2 efs, prim_step e1 σ1 e2 σ2 efs → σ1 = σ2) →
-  (|={E,E'}▷=> ∀ e2 efs σ, ⌜prim_step e1 σ e2 σ efs⌝ →
+  (∀ κ σ1 e2 σ2 efs, prim_step e1 σ1 κ e2 σ2 efs → κ = None /\ σ1 = σ2) →
+  (|={E,E'}▷=> ∀ κ e2 efs σ, ⌜prim_step e1 σ κ e2 σ efs⌝ →
     WP e2 @ s; E {{ Φ }} ∗ [∗ list] ef ∈ efs, WP ef @ s; ⊤ {{ _, True }})
   ⊢ WP e1 @ s; E {{ Φ }}.
 Proof.
@@ -59,8 +59,8 @@ Proof.
   iIntros (σ1) "Hσ". iMod "H".
   iMod fupd_intro_mask' as "Hclose"; last iModIntro; first by set_solver. iSplit.
   { iPureIntro. destruct s; done. }
-  iNext. iIntros (e2 σ2 efs ?).
-  destruct (Hstep σ1 e2 σ2 efs); auto; subst.
+  iNext. iIntros (κ e2 σ2 efs ?).
+  destruct (Hstep κ σ1 e2 σ2 efs); auto; subst.
   iMod "Hclose" as "_". iFrame "Hσ". iMod "H". iApply "H"; auto.
 Qed.
 
@@ -81,7 +81,7 @@ Lemma wp_lift_atomic_step_fupd {s E1 E2 Φ} e1 :
   to_val e1 = None →
   (∀ σ1, state_interp σ1 ={E1}=∗
     ⌜if s is NotStuck then reducible e1 σ1 else True⌝ ∗
-    ∀ e2 σ2 efs, ⌜prim_step e1 σ1 e2 σ2 efs⌝ ={E1,E2}▷=∗
+    ∀ κ e2 σ2 efs, ⌜prim_step e1 σ1 κ e2 σ2 efs⌝ ={E1,E2}▷=∗
       state_interp σ2 ∗
       from_option Φ False (to_val e2) ∗ [∗ list] ef ∈ efs, WP ef @ s; ⊤ {{ _, True }})
   ⊢ WP e1 @ s; E1 {{ Φ }}.
@@ -89,8 +89,8 @@ Proof.
   iIntros (?) "H". iApply (wp_lift_step_fupd s E1 _ e1)=>//; iIntros (σ1) "Hσ1".
   iMod ("H" $! σ1 with "Hσ1") as "[$ H]".
   iMod (fupd_intro_mask' E1 ∅) as "Hclose"; first set_solver.
-  iIntros "!>" (e2 σ2 efs ?). iMod "Hclose" as "_".
-  iMod ("H" $! e2 σ2 efs with "[#]") as "H"; [done|].
+  iIntros "!>" (κ e2 σ2 efs ?). iMod "Hclose" as "_".
+  iMod ("H" $! κ e2 σ2 efs with "[#]") as "H"; [done|].
   iMod (fupd_intro_mask' E2 ∅) as "Hclose"; [set_solver|]. iIntros "!> !>".
   iMod "Hclose" as "_". iMod "H" as "($ & HΦ & $)".
   destruct (to_val e2) eqn:?; last by iExFalso.
@@ -101,7 +101,7 @@ Lemma wp_lift_atomic_step {s E Φ} e1 :
   to_val e1 = None →
   (∀ σ1, state_interp σ1 ={E}=∗
     ⌜if s is NotStuck then reducible e1 σ1 else True⌝ ∗
-    ▷ ∀ e2 σ2 efs, ⌜prim_step e1 σ1 e2 σ2 efs⌝ ={E}=∗
+    ▷ ∀ κ e2 σ2 efs, ⌜prim_step e1 σ1 κ e2 σ2 efs⌝ ={E}=∗
       state_interp σ2 ∗
       from_option Φ False (to_val e2) ∗ [∗ list] ef ∈ efs, WP ef @ s; ⊤ {{ _, True }})
   ⊢ WP e1 @ s; E {{ Φ }}.
@@ -113,14 +113,14 @@ Qed.
 
 Lemma wp_lift_pure_det_step `{Inhabited (state Λ)} {s E E' Φ} e1 e2 efs :
   (∀ σ1, if s is NotStuck then reducible e1 σ1 else to_val e1 = None) →
-  (∀ σ1 e2' σ2 efs', prim_step e1 σ1 e2' σ2 efs' → σ1 = σ2 ∧ e2 = e2' ∧ efs = efs')→
+  (∀ σ1 κ e2' σ2 efs', prim_step e1 σ1 κ e2' σ2 efs' → κ = None /\ σ1 = σ2 ∧ e2 = e2' ∧ efs = efs')→
   (|={E,E'}▷=> WP e2 @ s; E {{ Φ }} ∗ [∗ list] ef ∈ efs, WP ef @ s; ⊤ {{ _, True }})
   ⊢ WP e1 @ s; E {{ Φ }}.
 Proof.
   iIntros (? Hpuredet) "H". iApply (wp_lift_pure_step s E E'); try done.
-  { by intros; eapply Hpuredet. }
+  { by naive_solver. }
   iApply (step_fupd_wand with "H"); iIntros "H".
-  by iIntros (e' efs' σ (_&->&->)%Hpuredet).
+  by iIntros (κ e' efs' σ (->&_&->&->)%Hpuredet).
 Qed.
 
 Lemma wp_pure_step_fupd `{Inhabited (state Λ)} s E E' e1 e2 φ Φ :
