theories/program_logic/total_lifting.v
@@ -15,7 +15,7 @@ Lemma twp_lift_step s E Φ e1 :
   to_val e1 = None →
   (∀ σ1, state_interp σ1 ={E,∅}=∗
     ⌜if s is NotStuck then reducible e1 σ1 else True⌝ ∗
-    ∀ e2 σ2 efs, ⌜prim_step e1 σ1 e2 σ2 efs⌝ ={∅,E}=∗
+    ∀ κ e2 σ2 efs, ⌜prim_step e1 σ1 κ e2 σ2 efs⌝ ={∅,E}=∗
       state_interp σ2 ∗ WP e2 @ s; E [{ Φ }] ∗ [∗ list] ef ∈ efs, WP ef @ s; ⊤ [{ _, True }])
   ⊢ WP e1 @ s; E [{ Φ }].
 Proof. by rewrite twp_unfold /twp_pre=> ->. Qed.
@@ -23,8 +23,8 @@ Proof. by rewrite twp_unfold /twp_pre=> ->. Qed.
 (** Derived lifting lemmas. *)
 Lemma twp_lift_pure_step `{Inhabited (state Λ)} s E Φ e1 :
   (∀ σ1, reducible e1 σ1) →
-  (∀ σ1 e2 σ2 efs, prim_step e1 σ1 e2 σ2 efs → σ1 = σ2) →
-  (|={E}=> ∀ e2 efs σ, ⌜prim_step e1 σ e2 σ efs⌝ →
+  (∀ σ1 κ e2 σ2 efs, prim_step e1 σ1 κ e2 σ2 efs → κ = None /\ σ1 = σ2) →
+  (|={E}=> ∀ κ e2 efs σ, ⌜prim_step e1 σ κ e2 σ efs⌝ →
     WP e2 @ s; E [{ Φ }] ∗ [∗ list] ef ∈ efs, WP ef @ s; ⊤ [{ _, True }])
   ⊢ WP e1 @ s; E [{ Φ }].
 Proof.
@@ -32,8 +32,8 @@ Proof.
   { eapply reducible_not_val, (Hsafe inhabitant). }
   iIntros (σ1) "Hσ". iMod "H".
   iMod fupd_intro_mask' as "Hclose"; last iModIntro; first set_solver.
-  iSplit; [by destruct s|]; iIntros (e2 σ2 efs ?).
-  destruct (Hstep σ1 e2 σ2 efs); auto; subst.
+  iSplit; [by destruct s|]; iIntros (κ e2 σ2 efs ?).
+  destruct (Hstep σ1 κ e2 σ2 efs); auto; subst.
   iMod "Hclose" as "_". iFrame "Hσ". iApply "H"; auto.
 Qed.
 
@@ -43,7 +43,7 @@ Lemma twp_lift_atomic_step {s E Φ} e1 :
   to_val e1 = None →
   (∀ σ1, state_interp σ1 ={E}=∗
     ⌜if s is NotStuck then reducible e1 σ1 else True⌝ ∗
-    ∀ e2 σ2 efs, ⌜prim_step e1 σ1 e2 σ2 efs⌝ ={E}=∗
+    ∀ κ e2 σ2 efs, ⌜prim_step e1 σ1 κ e2 σ2 efs⌝ ={E}=∗
       state_interp σ2 ∗
       from_option Φ False (to_val e2) ∗ [∗ list] ef ∈ efs, WP ef @ s; ⊤ [{ _, True }])
   ⊢ WP e1 @ s; E [{ Φ }].
@@ -51,21 +51,21 @@ Proof.
   iIntros (?) "H". iApply (twp_lift_step _ E _ e1)=>//; iIntros (σ1) "Hσ1".
   iMod ("H" $! σ1 with "Hσ1") as "[$ H]".
   iMod (fupd_intro_mask' E ∅) as "Hclose"; first set_solver.
-  iIntros "!>" (e2 σ2 efs) "%". iMod "Hclose" as "_".
-  iMod ("H" $! e2 σ2 efs with "[#]") as "($ & HΦ & $)"; first by eauto.
+  iIntros "!>" (κ e2 σ2 efs) "%". iMod "Hclose" as "_".
+  iMod ("H" $! κ e2 σ2 efs with "[#]") as "($ & HΦ & $)"; first by eauto.
   destruct (to_val e2) eqn:?; last by iExFalso.
   iApply twp_value; last done. by apply of_to_val.
 Qed.
 
 Lemma twp_lift_pure_det_step `{Inhabited (state Λ)} {s E Φ} e1 e2 efs :
   (∀ σ1, reducible e1 σ1) →
-  (∀ σ1 e2' σ2 efs', prim_step e1 σ1 e2' σ2 efs' → σ1 = σ2 ∧ e2 = e2' ∧ efs = efs')→
+  (∀ σ1 κ e2' σ2 efs', prim_step e1 σ1 κ e2' σ2 efs' → κ = None /\ σ1 = σ2 ∧ e2 = e2' ∧ efs = efs')→
   (|={E}=> WP e2 @ s; E [{ Φ }] ∗ [∗ list] ef ∈ efs, WP ef @ s; ⊤ [{ _, True }])
   ⊢ WP e1 @ s; E [{ Φ }].
 Proof.
   iIntros (? Hpuredet) ">H". iApply (twp_lift_pure_step _ E); try done.
-  { by intros; eapply Hpuredet. }
-  by iIntros "!>" (e' efs' σ (_&->&->)%Hpuredet).
+  { by naive_solver. }
+  by iIntros "!>" (κ e' efs' σ (->&_&->&->)%Hpuredet).
 Qed.
 
 Lemma twp_pure_step `{Inhabited (state Λ)} s E e1 e2 φ Φ :
